NLustre/NLSemanticsCoIndRec.v
@@ -1,0 +1,265 @@
+Require Import List.
+Import List.ListNotations.
+Open Scope list_scope.
+Require Import Coq.Sorting.Permutation.
+
+Require Import Coq.FSets.FMapPositive.
+Require Import Velus.Common.
+Require Import Velus.Operators.
+Require Import Velus.Clocks.
+Require Import Velus.NLustre.NLSyntax.
+Require Import Velus.NLustre.NLSemanticsCommon.
+Require Import Velus.NLustre.Ordered.
+Require Import Streams.
+
+(** * The NLustre semantics *)
+
+(**
+
+  We provide a "standard" dataflow semantics relating an environment
+  of streams to a stream of outputs.
+
+ *)
+
+Module Type NLSEMANTICSCOINDREC
+       (Import Ids   : IDS)
+       (Import Op    : OPERATORS)
+       (Import OpAux : OPERATORS_AUX Op)
+       (Import Clks  : CLOCKS    Ids)
+       (Import Syn   : NLSYNTAX  Ids Op Clks)
+       (Import Comm  : NLSEMANTICSCOMMON Ids Op OpAux Clks Syn)
+       (Import Ord   : ORDERED   Ids Op Clks Syn).
+
+  CoInductive fby1
+    : val -> val -> Stream value -> Stream value -> Prop :=
+  | Fby1A:
+      forall v c xs ys,
+        fby1 v c xs ys ->
+        fby1 v c (absent ::: xs) (absent ::: ys)
+  | Fby1P:
+      forall v x c xs ys,
+        fby1 x c xs ys ->
+        fby1 v c (present x ::: xs) (present v ::: ys)
+
+  with fby: val -> Stream value -> Stream value -> Prop :=
+  | FbyA:
+      forall c xs ys,
+        fby c xs ys ->
+        fby c (absent ::: xs) (absent ::: ys)
+  | FbyP:
+      forall x c xs ys,
+        fby1 x c xs ys ->
+        fby c (present x ::: xs) (present c ::: ys).
+
+  Definition reset_of : Stream value -> Stream value :=
+    map (fun x => match x with
+               | present x => if (x ==b true_val) then present x else present false_val
+               | _ => present false_val
+               end).
+
+  CoInductive true_s : Stream value -> Stream value -> Prop :=
+   | true_s_A:
+      forall xs ts,
+        true_s xs ts ->
+        true_s (absent ::: xs) (absent ::: ts)
+   | true_s_P:
+      forall x xs ts,
+        true_s xs ts ->
+        true_s (present x ::: xs) (present true_val ::: ts).
+
+  CoFixpoint true_s' (ss: Stream value) : Stream value :=
+    match ss with
+    | absent    ::: ss => absent ::: true_s' ss
+    | present _ ::: ss => present true_val ::: true_s' ss
+    end.
+
+  CoInductive once : Stream value -> Stream value -> Prop :=
+  | once_A:
+      forall bs ys,
+        once bs ys ->
+        once (absent ::: bs) (absent ::: ys)
+  | once_PF:
+      forall bs ys,
+        once bs ys ->
+        once (present false_val ::: bs) (present false_val ::: ys)
+  | once_PT:
+      forall bs ts,
+        true_s bs ts ->
+        once (present true_val ::: bs) ts.
+
+  CoFixpoint once' (ss: Stream value) : Stream value :=
+    match ss with
+    | absent ::: ss => absent ::: once' ss
+    | present s ::: ss =>
+      present s :::
+      if s ==b true_val then
+        true_s' ss
+      else
+        once' ss
+    end.
+
+  CoInductive switch : Stream value -> Stream value -> Stream value -> Stream value -> Prop :=
+  | switch_A:
+      forall bs xs ys zs,
+        switch bs xs ys zs ->
+        switch (absent ::: bs) (absent ::: xs) ys (absent ::: zs)
+  | switch_PF:
+      forall bs x xs ys zs,
+        switch bs xs ys zs ->
+        switch (present false_val ::: bs) (present x ::: xs) ys (present x ::: zs)
+  | switch_PT:
+      forall bs x xs ys,
+        switch (present true_val ::: bs) (present x ::: xs) ys ys.
+
+  Definition pre_ini (v0: val) (xs: Stream value) : Stream value :=
+    match xs with
+      x ::: xs => present v0 ::: xs
+    end.
+
+  Section NodeSemantics.
+
+    Variable G: global.
+
+    Inductive sem_equation: history -> Stream bool -> equation -> Prop :=
+    | SeqDef:
+        forall H b x ck e es,
+          sem_cexp H b e es ->
+          sem_var H x es ->
+          sem_equation H b (EqDef x ck e)
+    | SeqApp:
+        forall H b ys ck f es ess oss,
+          Forall2 (sem_lexp H b) es ess ->
+          sem_node f ess oss ->
+          Forall2 (sem_var H) ys oss ->
+          sem_equation H b (EqApp ys ck f es None)
+    | SeqReset:
+        forall H b ys ck f es x xs ess oss,
+          Forall2 (sem_lexp H b) es ess ->
+          sem_var H x xs ->
+          sem_reset f (reset_of xs) ess oss ->
+          Forall2 (sem_var H) ys oss ->
+          sem_equation H b (EqApp ys ck f es (Some x))
+    | SeqFby:
+        forall H b x ck c0 e es os,
+          sem_lexp H b e es ->
+          fby (sem_const c0) es os ->
+          sem_var H x os ->
+          sem_equation H b (EqFby x ck c0 e)
+
+    with sem_reset: ident -> Stream value -> list (Stream value) -> list (Stream value) -> Prop :=
+         | SReset:
+             forall f r once_r r' xss xss' yss rst oss,
+               sem_node f xss yss ->
+               once_r = once' r ->
+               Forall2 (fun xs xs' => when true xs once_r xs') xss xss' ->
+               when true r once_r r' ->
+               sem_reset f (pre_ini false_val r') xss' rst ->
+               Forall3 (switch r) yss rst oss ->
+               sem_reset f r xss oss
+
+    with sem_node: ident -> list (Stream value) -> list (Stream value) -> Prop :=
+         | SNode:
+             forall H f n xss oss,
+               find_node f G = Some n ->
+               Forall2 (sem_var H) (idents n.(n_in)) xss ->
+               Forall2 (sem_var H) (idents n.(n_out)) oss ->
+               Forall (sem_equation H (clocks_of xss)) n.(n_eqs) ->
+               sem_node f xss oss.
+
+  End NodeSemantics.
+
+  Section SemInd.
+
+    Variable G: global.
+
+    Variable P_equation: history -> Stream bool -> equation -> Prop.
+    Variable P_reset: ident -> Stream value -> list (Stream value) -> list (Stream value) -> Prop.
+    Variable P_node: ident -> list (Stream value) -> list (Stream value) -> Prop.
+
+    Hypothesis EqDefCase:
+      forall H b x ck e es,
+        sem_cexp H b e es ->
+        sem_var H x es ->
+        P_equation H b (EqDef x ck e).
+
+    Hypothesis EqAppCase:
+      forall H b ys ck f es ess oss,
+        Forall2 (sem_lexp H b) es ess ->
+        sem_node G f ess oss ->
+        Forall2 (sem_var H) ys oss ->
+        P_node f ess oss ->
+        P_equation H b (EqApp ys ck f es None).
+
+    Hypothesis EqResetCase:
+      forall H b ys ck f es x xs ess oss,
+        Forall2 (sem_lexp H b) es ess ->
+        sem_var H x xs ->
+        sem_reset G f (reset_of xs) ess oss ->
+        Forall2 (sem_var H) ys oss ->
+        P_reset f (reset_of xs) ess oss ->
+        P_equation H b (EqApp ys ck f es (Some x)).
+
+    Hypothesis EqFbyCase:
+      forall H b x ck c0 e es os,
+        sem_lexp H b e es ->
+        fby (sem_const c0) es os ->
+        sem_var H x os ->
+        P_equation H b (EqFby x ck c0 e).
+
+    Hypothesis ResetCase:
+      forall f r once_r r' xss xss' yss rst oss,
+        sem_node G f xss yss ->
+        once_r = once' r ->
+        Forall2 (fun xs xs' => when true xs once_r xs') xss xss' ->
+        when true r once_r r' ->
+        sem_reset G f (pre_ini false_val r') xss' rst ->
+        Forall3 (switch r) yss rst oss ->
+        P_node f xss yss ->
+        P_reset f (pre_ini false_val r') xss' rst ->
+        P_reset f r xss oss.
+
+    Hypothesis NodeCase:
+      forall H f n xss oss,
+        find_node f G = Some n ->
+        Forall2 (sem_var H) (idents n.(n_in)) xss ->
+        Forall2 (sem_var H) (idents n.(n_out)) oss ->
+        Forall (sem_equation G H (clocks_of xss)) n.(n_eqs) ->
+        Forall (P_equation H (clocks_of xss)) n.(n_eqs) ->
+        P_node f xss oss.
+
+    Fixpoint sem_equation_mult
+             (H: history) (b: Stream bool) (e: equation)
+             (Sem: sem_equation G H b e) {struct Sem}
+      : P_equation H b e
+    with sem_reset_mult
+           (f: ident) (r: Stream value) (xss oss: list (Stream value))
+           (Sem: sem_reset G f r xss oss) {struct Sem}
+         : P_reset f r xss oss
+    with sem_node_mult
+           (f: ident) (xss oss: list (Stream value))
+           (Sem: sem_node G f xss oss) {struct Sem}
+         : P_node f xss oss.
+    Proof.
+      - destruct Sem; eauto.
+      - destruct Sem; eauto.
+      - destruct Sem; eauto.
+        eapply NodeCase; eauto.
+        induction H3; auto.
+    Qed.
+
+    Combined Scheme sem_equation_node_ind from sem_equation_mult, sem_node_mult, sem_reset_mult.
+
+  End SemInd.
+
+End NLSEMANTICSCOINDREC.
+
+(* Module NLSemanticsCoIndRecFun *)
+(*        (Ids   : IDS) *)
+(*        (Op    : OPERATORS) *)
+(*        (OpAux : OPERATORS_AUX Op) *)
+(*        (Clks  : CLOCKS    Ids) *)
+(*        (Syn   : NLSYNTAX  Ids Op Clks) *)
+(*        (Ord   : ORDERED   Ids Op Clks Syn) *)
+(*        <: NLSEMANTICSCOINDREC Ids Op OpAux Clks Syn Ord. *)
+(*   Include NLSEMANTICSCOINDREC Ids Op OpAux Clks Syn Ord. *)
+(* End NLSemanticsCoIndRecFun. *)
