NLustre/NLSemanticsCoIndWire.v
@@ -1,0 +1,190 @@
+Require Import List.
+Import List.ListNotations.
+Open Scope list_scope.
+Require Import Coq.Sorting.Permutation.
+
+Require Import Coq.FSets.FMapPositive.
+Require Import Velus.Common.
+Require Import Velus.Operators.
+Require Import Velus.Clocks.
+Require Import Velus.NLustre.NLSyntax.
+Require Import Velus.NLustre.NLSemanticsCommon.
+Require Import Velus.NLustre.Ordered.
+Require Import Streams.
+
+(** * The NLustre semantics *)
+
+(**
+
+  We provide a "standard" dataflow semantics relating an environment
+  of streams to a stream of outputs.
+
+ *)
+
+Module Type NLSEMANTICSCOINDWIRE
+       (Import Ids   : IDS)
+       (Import Op    : OPERATORS)
+       (Import OpAux : OPERATORS_AUX Op)
+       (Import Clks  : CLOCKS    Ids)
+       (Import Syn   : NLSYNTAX  Ids Op Clks)
+       (Import Comm  : NLSEMANTICSCOMMON Ids Op OpAux Clks Syn)
+       (Import Ord   : ORDERED   Ids Op Clks Syn).
+
+  CoInductive fby1
+    : Stream bool -> val -> val -> Stream value -> Stream value -> Prop :=
+  | Fby1ANR:
+      forall rs v c xs ys,
+        fby1 rs v c xs ys ->
+        fby1 (false ::: rs) v c (absent ::: xs) (absent ::: ys)
+  | Fby1AR:
+      forall rs v c xs ys,
+        fby rs c xs ys ->
+        fby1 (true ::: rs) v c (absent ::: xs) (absent ::: ys)
+  | Fby1PNR:
+      forall rs v x c xs ys,
+        fby1 rs x c xs ys ->
+        fby1 (false ::: rs) v c (present x ::: xs) (present v ::: ys)
+  | Fby1PR:
+      forall rs v x c xs ys,
+        fby1 rs x c xs ys ->
+        fby1 (true ::: rs) v c (present x ::: xs) (present c ::: ys)
+
+  with fby: Stream bool -> val -> Stream value -> Stream value -> Prop :=
+  | FbyA:
+      forall r rs c xs ys,
+        fby rs c xs ys ->
+        fby (r ::: rs) c (absent ::: xs) (absent ::: ys)
+  | FbyP:
+      forall r rs x c xs ys,
+        fby1 rs x c xs ys ->
+        fby (r ::: rs) c (present x ::: xs) (present c ::: ys).
+
+  CoFixpoint reset_of : Stream value -> Stream bool :=
+    map (fun x => match x with
+               | present x => x ==b true_val
+               | _ => false
+               end).
+
+  CoFixpoint merge_reset (rs rs' : Stream bool) : Stream bool :=
+    match rs, rs' with
+      r ::: rs, r' ::: rs' => r || r' ::: merge_reset rs rs'
+    end.
+
+  Section NodeSemantics.
+
+    Variable G: global.
+
+    Inductive sem_equation: history -> Stream bool -> Stream bool -> equation -> Prop :=
+    | SeqDef:
+        forall H b r x ck e es,
+          sem_cexp H b e es ->
+          sem_var H x es ->
+          sem_equation H b r (EqDef x ck e)
+    | SeqApp:
+        forall H b r ys ck f es ess oss,
+          Forall2 (sem_lexp H b) es ess ->
+          sem_node r f ess oss ->
+          Forall2 (sem_var H) ys oss ->
+          sem_equation H b r (EqApp ys ck f es None)
+    | SeqReset:
+        forall H b r ys ck f es x rs ess oss,
+          Forall2 (sem_lexp H b) es ess ->
+          sem_var H x rs ->
+          sem_node (merge_reset r (reset_of rs)) f ess oss ->
+          Forall2 (sem_var H) ys oss ->
+          sem_equation H b r (EqApp ys ck f es (Some x))
+    | SeqFby:
+        forall H b r x ck c0 e es os,
+          sem_lexp H b e es ->
+          fby r (sem_const c0) es os ->
+          sem_var H x os ->
+          sem_equation H b r (EqFby x ck c0 e)
+
+    with sem_node: Stream bool -> ident -> list (Stream value) -> list (Stream value) -> Prop :=
+         | SNode:
+             forall H r f n xss oss,
+               find_node f G = Some n ->
+               Forall2 (sem_var H) (idents n.(n_in)) xss ->
+               Forall2 (sem_var H) (idents n.(n_out)) oss ->
+               Forall (sem_equation H (clocks_of xss) r) n.(n_eqs) ->
+               sem_node r f xss oss.
+
+  End NodeSemantics.
+
+  Section SemInd.
+
+    Variable G: global.
+
+    Variable P_equation: history -> Stream bool -> Stream bool -> equation -> Prop.
+    Variable P_node: Stream bool -> ident -> list (Stream value) -> list (Stream value) -> Prop.
+
+    Hypothesis EqDefCase:
+      forall H b r x ck e es,
+        sem_cexp H b e es ->
+        sem_var H x es ->
+        P_equation H b r (EqDef x ck e).
+
+    Hypothesis EqAppCase:
+      forall H b r ys ck f es ess oss,
+        Forall2 (sem_lexp H b) es ess ->
+        sem_node G r f ess oss ->
+        Forall2 (sem_var H) ys oss ->
+        P_node r f ess oss ->
+        P_equation H b r (EqApp ys ck f es None).
+
+    Hypothesis EqResetCase:
+      forall H b r ys ck f es x rs ess oss,
+        Forall2 (sem_lexp H b) es ess ->
+        sem_node G (merge_reset r (reset_of rs)) f ess oss ->
+        sem_var H x rs ->
+        Forall2 (sem_var H) ys oss ->
+        P_node (merge_reset r (reset_of rs)) f ess oss ->
+        P_equation H b r (EqApp ys ck f es (Some x)).
+
+    Hypothesis EqFbyCase:
+      forall H b r x ck c0 e es os,
+        sem_lexp H b e es ->
+        fby r (sem_const c0) es os ->
+        sem_var H x os ->
+        P_equation H b r (EqFby x ck c0 e).
+
+    Hypothesis NodeCase:
+      forall H r f n xss oss,
+        find_node f G = Some n ->
+        Forall2 (sem_var H) (idents n.(n_in)) xss ->
+        Forall2 (sem_var H) (idents n.(n_out)) oss ->
+        Forall (sem_equation G H (clocks_of xss) r) n.(n_eqs) ->
+        Forall (P_equation H (clocks_of xss) r) n.(n_eqs) ->
+        P_node r f xss oss.
+
+    Fixpoint sem_equation_mult
+             (H: history) (b r: Stream bool) (e: equation)
+             (Sem: sem_equation G H b r e) {struct Sem}
+      : P_equation H b r e
+    with sem_node_mult
+           (r: Stream bool) (f: ident) (xss oss: list (Stream value))
+           (Sem: sem_node G r f xss oss) {struct Sem}
+         : P_node r f xss oss.
+    Proof.
+      - destruct Sem; eauto.
+      - destruct Sem; eauto.
+        eapply NodeCase; eauto.
+        induction H3; auto.
+    Qed.
+
+    Combined Scheme sem_equation_node_ind from sem_equation_mult, sem_node_mult.
+
+  End SemInd.
+
+End NLSEMANTICSCOINDWIRE.
+
+(* Module NLSemanticsCoIndWireFun *)
+(*        (Ids   : IDS) *)
+(*        (Op    : OPERATORS) *)
+(*        (OpAux : OPERATORS_AUX Op) *)
+(*        (Clks  : CLOCKS    Ids) *)
+(*        (Syn   : NLSYNTAX  Ids Op Clks) *)
+(*        (Ord   : ORDERED   Ids Op Clks Syn) *)
+(*        <: NLSEMANTICSCOINDWIRE Ids Op OpAux Clks Syn Ord. *)
+(*   Include NLSEMANTICSCOINDWIRE Ids Op OpAux Clks Syn Ord. *)
+(* End NLSemanticsCoIndWireFun. *)
