NLustre/SemEquiv.v
@@ -1,0 +1,176 @@
+Require Import List.
+Import List.ListNotations.
+Open Scope list_scope.
+Require Import Coq.Sorting.Permutation.
+
+Require Import Coq.FSets.FMapPositive.
+Require Import Velus.Common.
+Require Import Velus.Operators.
+Require Import Velus.Clocks.
+Require Import Velus.NLustre.NLSyntax.
+Require Import Velus.NLustre.NLSemanticsCommon.
+Require Import Velus.NLustre.Ordered.
+Require Import Streams.
+
+Require Import Velus.NLustre.NLSemanticsCoIndWire.
+Require Import Velus.NLustre.NLSemanticsCoIndRec.
+
+Module Type SEMEQUIV
+       (Import Ids   : IDS)
+       (Import Op    : OPERATORS)
+       (Import OpAux : OPERATORS_AUX Op)
+       (Import Clks  : CLOCKS    Ids)
+       (Import Syn   : NLSYNTAX  Ids Op Clks)
+       (Import Comm  : NLSEMANTICSCOMMON Ids Op OpAux Clks Syn)
+       (Import Ord   : ORDERED   Ids Op Clks Syn)
+       (Wire  : NLSEMANTICSCOINDWIRE Ids Op OpAux Clks Syn Comm Ord)
+       (Rec   : NLSEMANTICSCOINDREC  Ids Op OpAux Clks Syn Comm Ord).
+
+  CoFixpoint false_s : Stream bool := false ::: false_s.
+
+  Lemma unfold_false_s : false_s = false ::: false_s.
+  Proof.
+    rewrite unfold_Stream at 1; auto.
+  Qed.
+
+  Section Global.
+
+    Variable G: global.
+
+    Lemma fby1_equiv:
+      forall c v xs ys,
+        Wire.fby1 false_s v (sem_const c) xs ys <->
+        Rec.fby1 v (sem_const c) xs ys.
+    Proof.
+      split; revert c v xs ys; cofix CoFby1; intros ** Fby1.
+      - rewrite unfold_false_s in Fby1.
+        inversion Fby1; constructor; auto.
+      - rewrite unfold_false_s.
+        inversion Fby1; constructor; auto.
+    Qed.
+
+    Lemma fby_equiv:
+      forall c xs ys,
+        Wire.fby false_s (sem_const c) xs ys <->
+        Rec.fby (sem_const c) xs ys.
+    Proof.
+      split; revert xs ys; cofix CoFby; intros ** Fby.
+      - rewrite unfold_false_s in Fby.
+        inversion_clear Fby; constructor; auto.
+        now apply fby1_equiv.
+      - rewrite unfold_false_s.
+        inversion_clear Fby; constructor; auto.
+        now apply fby1_equiv.
+    Qed.
+
+    CoInductive synchronised: Stream value -> Stream value -> Prop :=
+    | A_synchro:
+        forall xs ys,
+          synchronised xs ys ->
+          synchronised (absent ::: xs) (absent ::: ys)
+    | P_synchro:
+        forall xs ys x y,
+          synchronised xs ys ->
+          synchronised (present x ::: xs) (present y ::: ys).
+
+    Ltac prove_synchro :=
+      match goal with
+        |- forall s, synchronised s ?s' =>
+        let COFIX := fresh "COFIX" in
+        let s := fresh s in
+        let v := fresh "v" in
+        cofix COFIX; intro s;
+        rewrite unfold_Stream;
+        destruct s as [v]; destruct v; simpl; constructor; auto
+      end.
+
+    Lemma true_s'_synchronised:
+      forall s, synchronised s (Rec.true_s' s).
+    Proof. prove_synchro. Qed.
+
+    Lemma once'_synchronised:
+      forall s, synchronised s (Rec.once' s).
+    Proof.
+      prove_synchro.
+      destruct (c ==b true_val); auto.
+      apply true_s'_synchronised.
+    Qed.
+
+    Lemma when_witness:
+      forall k xs ys,
+        synchronised xs ys ->
+        exists rs, when k xs ys rs.
+    Proof.
+      eexists.
+      revert k xs ys H.
+      cofix.
+      intros.
+      inv H.
+      - constructor.
+    Admitted.
+
+    Lemma WireRec_node_reset:
+      forall rs f ess oss,
+        Wire.sem_node G (Wire.merge_reset false_s (Wire.reset_of rs)) f ess oss ->
+        Rec.sem_node G f ess oss ->
+        Rec.sem_reset G f (Rec.reset_of rs) ess oss.
+    Proof.
+      intros ** Reset Node.
+      destruct Reset.
+
+      assert (exists xss', Forall2 (fun xs xs' => when true xs (Rec.once' (Rec.reset_of rs)) xs') xss xss')
+        as (xss' & When_xss).
+      { clear; induction xss.
+        - eexists; eauto.
+        - edestruct IHxss.
+          edestruct (when_witness true a (Rec.once' (Rec.reset_of rs))).
+          admit.
+          eexists.
+          constructor; eauto.
+      }
+
+      assert (exists rs', when true (Rec.reset_of rs) (Rec.once' (Rec.reset_of rs)) rs')
+        as (rs' & When_rs) by apply when_witness, once'_synchronised.
+
+       econstructor; eauto.
+      - clear; induction xss.
+        + eexists; eauto.
+
+    Admitted.
+
+    Lemma WireRec_equation_node:
+      (forall H b r e,
+          Wire.sem_equation G H b r e ->
+          (* r = false_s -> *)
+          Rec.sem_equation G H b e)
+      /\
+      (forall r f xss oss,
+          Wire.sem_node G r f xss oss ->
+          Rec.sem_node G f xss oss).
+    Proof.
+      Check Wire.sem_equation_node_ind.
+      apply Wire.sem_equation_node_ind; intros.
+      - econstructor; eauto.
+      - econstructor; eauto.
+      - econstructor; eauto.
+        eapply WireRec_node_reset; eauto.
+      - econstructor; eauto.
+        subst; now apply fby_equiv.
+      - econstructor; eauto.
+        apply Forall_impl with (2:=H4).
+        auto.
+    Qed.
+
+    Theorem WireRec:
+      forall G f xss yss,
+        Wire.sem_node G false_s f xss yss
+        <-> Rec.sem_node G f xss yss.
+    Proof.
+      split; intro Sem; inv Sem; econstructor; eauto; eapply Forall_impl;
+        [ now apply WireRec_equation | auto
+          | now apply WireRec_equation | auto ].
+    Qed.
+
+    SearchAbout Forall.
+
+  End SEMEQUIV.
